Migrate the remaining staged invariant files and redefine wp_nval using private invariants.

src/program_logic/wp_nval.v
@@ -3,12 +3,59 @@ From Perennial.program_logic Require Export crash_weakestpre staged_invariant_al
 Set Default Proof Using "Type".
 Import uPred.
 
+Definition logical_step_emp `{!irisGS Λ Σ, !crashGS Σ} E D P : iProp Σ :=
+  ∀ Q, (|={E|D}⧗=> Q) -∗ (|={E|D}⧗=> Q ∗ P).
+Notation "|~{ E | D }~> P" := (logical_step_emp E D P) (at level 99, P at level 200, format "'[  ' |~{ E | D }~>  '/' P ']'").
+
+Lemma logical_step_emp_wand `{!irisGS Λ Σ, !crashGS Σ} E D P Q :
+  (|~{E|D}~> P) -∗  
+  (P -∗ Q) -∗
+  |~{E|D}~> Q.
+Proof.
+  iIntros "Hstep HPQ" (R) "HR".
+  iDestruct ("Hstep" with "HR") as "HR".
+  iApply (physical_step_wand with "HR"). iIntros "[$ P]".
+  by iApply "HPQ".
+Qed.
+
+Lemma logical_step_emp_intro `{!irisGS Λ Σ, !crashGS Σ} E D P :
+  P -∗
+  |~{E|D}~> P.
+Proof.
+  iIntros "HP" (R) "HR".
+  iApply (physical_step_wand with "HR"). by iIntros "$".
+Qed.
+
+Lemma logical_step_emp_use_tr_simpl `{!irisGS Λ Σ, !crashGS Σ} E D P n :
+  ⧗ n -∗
+  (|~{E|D}~> ⧗ (f n) -∗ £ (f n) -∗ P) -∗
+  |~{E|D}~> P.
+Proof.
+  iIntros "H⧗ Hstep" (R) "HR".
+  iDestruct ("Hstep" with "HR") as "HR".
+  iApply (physical_step_tr_use with "[$]").
+  iApply (physical_step_wand with "[$]").
+  iIntros "($&HP) H⧗ H£".
+  by iApply ("HP" with "[$] [$]").
+Qed.
+
+Lemma logical_step_apply `{!irisGS Λ Σ, !crashGS Σ} E D P Q :
+  (|~{E|D}~> P) -∗
+  (|={E|D}⧗=> P -∗ Q) -∗
+  |={E|D}⧗=> Q.
+Proof.
+  iIntros "Hstep HPQ".
+  iApply (physical_step_wand with "(Hstep HPQ)").
+  iIntros "[HPQ HP]". by iApply "HPQ".
+Qed.
+
 Definition wp_nval `{!irisGS Λ Σ, !crashGS Σ} E1 P :=
-  ((∀ mj q g1 ns D κs,
-       let E2 :=  ⊤ ∖ D in
-       let E2 :=  ⊤ ∖ D in
-       global_state_interp g1 ns mj D κs -∗ NC q -∗
-     ||={E1|E2,∅|∅}=> ||▷=>^(S (num_laters_per_step ns)) ||={∅|∅,E1|E2}=> global_state_interp g1 ns mj D κs ∗ P ∗ NC q))%I.
+  ((∀ mj q g1 D κs,
+       global_state_interp g1 mj D κs -∗ NC q -∗ ||={E1|⊤∖D, ∅|∅}=> ∃ D', ||={∅|∅, E1|⊤∖D'}=>
+       ∃ mj', ⌜mj' = mj ∨ (/2 < mj' ≤ mj)%Qp⌝ ∗ global_state_interp g1 mj' D' κs ∗ NC q ∗
+        |~{E1|⊤∖D'}~>
+          ∀ g1' κs', global_state_interp g1' mj' D' κs' -∗ NC q -∗ ||={E1|⊤∖D', E1|⊤∖D}=>
+            global_state_interp g1' mj D κs' ∗ P ∗ NC q))%I.
 
 Section modality.
 Context `{IRISG: !irisGS Λ Σ, !generationGS Λ Σ}.
@@ -19,27 +66,29 @@ Lemma wp_nval_strong_mono E P P' :
   wp_nval E P'.
 Proof.
   iIntros "Hwp_nval Hwand".
-  rewrite /wp_nval. iIntros (??????) "H HNC".
-  iSpecialize ("Hwp_nval" with "[$] [$]").
-  iApply (step_fupd2N_inner_fupd).
-  iApply (step_fupd2N_inner_wand with "Hwp_nval"); auto.
-  iIntros "($&HP&HNC)".
+  rewrite /wp_nval. iIntros (?????) "H HNC".
+  iMod ("Hwp_nval" with "[$] [$]") as (?) "H".
+  iModIntro. iExists _. iMod "H" as (?) "($&$&$&Hstep)".
+  iModIntro. iApply (logical_step_emp_wand with "[$]").
+  iIntros "Hstep" (??) "Hg HNC".
+  iMod ("Hstep" with "[$] [$]") as "($&HP&HNC)".
   rewrite ncfupd_eq /ncfupd_def. by iMod ("Hwand" with "[$] [$]") as "$".
-Qed.
-
-Lemma wp_nval_True E : ⊢ wp_nval E True%I.
-Proof.
-  rewrite /wp_nval. iIntros (??????) "H HNC".
-  iApply step_fupd2N_inner_later; auto. iNext.
-  iFrame.
 Qed.
 
 Lemma wp_nval_intro E P :
   P -∗ wp_nval E P.
 Proof.
-  iIntros "HP".
-  iPoseProof (wp_nval_True) as "Htrue".
-  iApply (wp_nval_strong_mono with "Htrue"); eauto.
+  rewrite /wp_nval. iIntros "HP" (?????) "H $".
+  iMod (fupd2_mask_subseteq ∅ ∅) as "Hclo"; [set_solver..|].
+  iFrame "H". iModIntro. iMod "Hclo". iModIntro.
+  iSplitR; first (iPureIntro; by left).
+  iApply logical_step_emp_intro.
+  iIntros (??) "$ $". by iFrame.
+Qed.
+
+Lemma wp_nval_True E : ⊢ wp_nval E True%I.
+Proof.
+  by iApply wp_nval_intro.
 Qed.
 
 Lemma wp_nval_ncfupd E P :
@@ -53,7 +102,7 @@ Lemma ncfupd_wp_nval E P :
   (|NC={E}=> wp_nval E P) -∗ wp_nval E P.
 Proof.
   iIntros "HP".
-  rewrite /wp_nval. iIntros (??????) "H HNC".
+  rewrite /wp_nval. iIntros (?????) "H HNC".
   iIntros. rewrite ncfupd_eq.
   iSpecialize ("HP" with "[$]").
   iMod (fupd_mask_mono with "HP") as "(HP&HNC)"; auto.
@@ -61,44 +110,60 @@ Proof.
 Qed.
 
 
-Context `{!later_tokG IRISG}.
+Context `{!later_tokG IRISG} `{!pri_invG IRISG}.
+
+Lemma wpc0_mj_le' E s mj1 mj2 e Φ Φc:
+  (mj1 = mj2 ∨ /2 < mj1 ≤ mj2)%Qp →
+  wpc0 s mj1 E e Φ Φc -∗
+  wpc0 s mj2 E e Φ Φc.
+Proof using pri_invG0.
+  destruct 1 as [->|H]; [eauto|].
+  by apply wpc0_mj_le.
+Qed.
+
 Lemma wp_nval_wpc_nval E P :
   later_tok -∗
   ▷ wp_nval E (later_tok -∗ P) -∗
   wpc_nval E P.
-Proof.
-  rewrite /wp_nval/wpc_nval. iIntros "Htok H" (E' e s Φ Φc Hnval Hsub) "Hwp".
+Proof using later_tokG0 pri_invG0.
+  iIntros "[H⧗ H£] Hval" (E' e s Φ Φc Hnval Hsub) "Hwp".
+  rewrite /wp_nval/wpc_nval.
   rewrite ?wpc_unfold /wpc_pre. iIntros (mj).
   rewrite Hnval. iSplit; last first.
   { iDestruct ("Hwp" $! _) as "(_&$)". }
-  iIntros (q σ1 g1 ns D κ κs nt) "Hσ Hg HNC Hlc".
-  iDestruct ("Hwp" $! mj) as "(Hwp&_)".
-  iMod (later_tok_decr with "[$]") as (ns' Hle) "Hg".
-  iMod (fupd2_mask_subseteq ∅ ∅) as "Hclo'"; [set_solver+..|].
+  iIntros (q σ1 g1 D κ κs nt) "Hσ Hg HNC".
+  iSplit. { iDestruct ("Hwp" $! mj) as "(Hwp&_)". iDestruct ("Hwp" with "[$] [$] [$]") as "[$ _]". }
+  iIntros.
+  iApply (physical_step_atomic E (⊤ ∖ D)).
+  iMod (fupd_mask_subseteq E) as "Hclo"; [done..|].
+  iApply (lc_fupd2_add_laterN with "[$]"). iNext. iNext. iModIntro.
+  iMod ("Hval" with "[$] [$]") as (?) ">Hstep".
+  iDestruct "Hstep" as (?) "(%Heq&Hg&HNC&Hstep)".
+  iDestruct ("Hwp" $! mj') as "(Hwp&_)".
+  iDestruct ("Hwp" with "[$] [$] [$] [//]") as "H".
+  iApply (logical_step_apply with "Hstep").
+  iApply (physical_step_atomic E' (⊤∖D')). iMod "Hclo" as "_".
   iModIntro.
-  simpl. iModIntro. iNext. iModIntro.
-  iApply (step_fupd2N_le).
-  { apply (num_laters_per_step_exp ns'). lia. }
-  iApply (step_fupd2N_le ((S (num_laters_per_step ns')) + S (num_laters_per_step ns'))).
-  { lia. }
-  simpl. rewrite Nat.iter_add.
-  iMod "Hclo'" as "_".
-  iMod (fupd2_mask_subseteq E (⊤ ∖ D)) as "Hclo'"; try set_solver.
-  iMod ("H" with "[$] [$]") as "H".
-  iApply (step_fupd2N_wand with "H"). iNext. iIntros "H".
-  simpl. iMod "H". iMod "Hclo'".
-  iDestruct "H" as "(Hg&HP&HNC)".
-  iMod ("Hwp" with "[$] [$] [$] [Hlc]") as "Hwp".
-  { iApply (lc_weaken with "Hlc").
-    apply num_laters_per_step_lt in Hle. lia. }
-  iApply (step_fupd2N_wand with "Hwp"). iNext. iIntros "($&Hwp)".
-  iIntros. iMod ("Hwp" with "[//]") as "($&Hg&Hwp&$)".
-  iMod (later_tok_incr with "[$]") as "(Hg&Htok)".
-  iMod (global_state_interp_le with "[$]") as "$".
-  { specialize (step_count_next_mono ns' ns). lia. }
-  iModIntro. iSpecialize ("HP" with "[$]").
-  iApply (wpc0_strong_mono with "Hwp"); auto. iSplit; last eauto.
-  iIntros (?) "HΦ". iModIntro. by iApply "HΦ".
+  iApply (physical_step_tr_use with "[$]").
+  iApply (physical_step_wand with "H").
+  iIntros "(Hσ & Hg & Hwpc & Hfork & HNC) H⧗ H£ !>".
+  iMod (fupd_mask_subseteq E) as "Hclo"; [done..|].
+  iModIntro. iIntros "Hnval".
+  iMod (fupd2_mask_subseteq ∅ ∅) as "Hclo'"; [set_solver..|].
+  iModIntro. iMod "Hclo'" as "_".
+  iMod ("Hnval" with "[$] [$]") as "(Hg&HP&HNC)". iModIntro.
+  iMod "Hclo" as "_". iModIntro. iFrame.
+  iSplitR "Hfork".
+  - iApply (wpc0_mj_le'); first done.
+    iApply (wpc0_strong_mono with "Hwpc"); auto. iSplit; last eauto.
+    iIntros (?) "HΦ". iModIntro. iApply "HΦ". iApply "HP".
+    assert (2 ≤ f 2).
+    { pose proof (f_exp 2); lia. }
+    iDestruct (lc_weaken with "[$]") as "$"; first done.
+    by iDestruct (tr_weaken with "[$]") as "$".
+  - iApply (big_sepL_mono with "[$]").
+    iIntros (???) "Hwpc".
+    by iApply (wpc0_mj_le').
 Qed.
 
 End modality.
